Switch to NoNode representation
Switching back to the NoNode alternative for NoNode but using
a slightly different approach using type lifting more extensively.

Canonicalization.thy
@@ -4,33 +4,32 @@ theory Canonicalization
   imports 
     IRGraphFrames
     IRStepObj
-    
 begin
 
 
 lemma eval_const_node:
-  assumes xn: "kind g x = Some (ConstantNode xv)"
-  shows "g m \<turnstile> x (the (kind g x)) \<mapsto> (IntVal xv)"
+  assumes xn: "kind g x = (ConstantNode xv)"
+  shows "g m \<turnstile> x (kind g x) \<mapsto> (IntVal xv)"
   using xn eval.ConstantNode by simp
 
 lemma eval_add_node: 
-  assumes x: "g m \<turnstile> x (the (kind g x)) \<mapsto> IntVal(xv)"
-  assumes y: "g m \<turnstile> y (the (kind g y)) \<mapsto> IntVal(yv)"
+  assumes x: "g m \<turnstile> x (kind g x) \<mapsto> IntVal(xv)"
+  assumes y: "g m \<turnstile> y (kind g y) \<mapsto> IntVal(yv)"
   shows "g m \<turnstile> z (AddNode x y) \<mapsto> IntVal(xv+yv)"
   using eval.AddNode x y by blast
 
 lemma add_const_nodes:
-  assumes xn: "kind g x = Some (ConstantNode xv)"
-  assumes yn: "kind g y = Some (ConstantNode yv)"
-  assumes zn: "kind g z = Some (AddNode x y)"
-  assumes wn: "kind g w = Some (ConstantNode (xv+yv))"
-  assumes ez: "g m \<turnstile> z (the (kind g z)) \<mapsto> (IntVal v1)"
-  assumes ew: "g m \<turnstile> w (the (kind g w)) \<mapsto> (IntVal v2)"
+  assumes xn: "kind g x = (ConstantNode xv)"
+  assumes yn: "kind g y = (ConstantNode yv)"
+  assumes zn: "kind g z = (AddNode x y)"
+  assumes wn: "kind g w = (ConstantNode (xv+yv))"
+  assumes ez: "g m \<turnstile> z (kind g z) \<mapsto> (IntVal v1)"
+  assumes ew: "g m \<turnstile> w (kind g w) \<mapsto> (IntVal v2)"
   shows "v1 = v2"
 proof -
-  have zv: "g m \<turnstile> z (the (kind g z)) \<mapsto> IntVal(xv+yv)"
+  have zv: "g m \<turnstile> z (kind g z) \<mapsto> IntVal(xv+yv)"
     using eval.AddNode eval_const_node xn yn zn by simp
-  have wv: "g m \<turnstile> w (the (kind g w)) \<mapsto> IntVal(xv+yv)"
+  have wv: "g m \<turnstile> w (kind g w) \<mapsto> IntVal(xv+yv)"
     using eval_const_node wn by auto
   show ?thesis using evalDet zv wv
     using ew ez by blast
@@ -39,13 +38,13 @@ qed
 text_raw \<open>\Snip{CreateAddNode}%\<close>
 fun create_add :: "IRGraph \<Rightarrow> ID \<Rightarrow> ID \<Rightarrow> IRNode" where 
   "create_add g x y = 
-    (case the (kind g x) of 
+    (case (kind g x) of 
       ConstantNode xv \<Rightarrow> 
-        (case the (kind g y) of
+        (case (kind g y) of
           ConstantNode yv \<Rightarrow> ConstantNode (xv+yv) | 
           _ \<Rightarrow> if xv = 0 then RefNode y else AddNode x y
         ) |
-      _ \<Rightarrow> (case the (kind g y) of
+      _ \<Rightarrow> (case (kind g y) of
             ConstantNode yv \<Rightarrow> 
               if yv = 0 then RefNode x else AddNode x y |
             _ \<Rightarrow> AddNode x y
@@ -56,8 +55,8 @@ text_raw \<open>\EndSnip\<close>
 
 text_raw \<open>\Snip{AddNodeCreate}%\<close>
 lemma add_node_create:
-  assumes xv: "g m \<turnstile> x (the (kind g x)) \<mapsto> IntVal(xv)"
-  assumes yv: "g m \<turnstile> y (the (kind g y)) \<mapsto> IntVal(yv)"
+  assumes xv: "g m \<turnstile> x (kind g x) \<mapsto> IntVal(xv)"
+  assumes yv: "g m \<turnstile> y (kind g y) \<mapsto> IntVal(yv)"
   shows 
     "(g m \<turnstile> nid (AddNode x y) \<mapsto> IntVal(xv+yv)) \<and>
      (g m \<turnstile> nid (create_add g x y) \<mapsto> IntVal(xv+yv))"
@@ -67,10 +66,10 @@ proof -
   have P: ?P
     using xv yv eval.AddNode by simp
   have Q: ?Q
-  proof (cases "\<exists>v. the (kind g x) = ConstantNode v")
+  proof (cases "\<exists>v. (kind g x) = ConstantNode v")
     case xconst: True
     then show ?thesis
-    proof (cases "\<exists>v. the (kind g y) = ConstantNode v")
+    proof (cases "\<exists>v. (kind g y) = ConstantNode v")
       case yconst: True
       then show ?thesis unfolding create_add.simps 
         using xconst eval.ConstantNode xv yv by auto
@@ -78,7 +77,8 @@ proof -
     next
       case ynotconst: False
       have "create_add g x y = (if xv = 0 then RefNode y else AddNode x y)"
-        using xconst ynotconst create_add.simps sorry
+        unfolding create_add.simps 
+        using xconst ynotconst sorry
       then show ?thesis unfolding create_add.simps
         apply (cases "xv = 0"; auto)
         using eval.RefNode yv apply simp
@@ -87,7 +87,7 @@ proof -
   next
     case xnotconst: False
     then show ?thesis
-    proof (cases "\<exists>v. the (kind g y) = ConstantNode v")
+    proof (cases "\<exists>v. (kind g y) = ConstantNode v")
       case yconst: True
       have "create_add g x y = (if yv = 0 then RefNode x else AddNode x y)"
         using xnotconst yconst create_add.simps sorry
@@ -111,7 +111,7 @@ text_raw \<open>\Snip{CreateIfNode}%\<close>
 fun create_if :: "IRGraph \<Rightarrow> ID \<Rightarrow> ID \<Rightarrow> ID \<Rightarrow> IRNode"
   where 
   "create_if g cond tb fb = 
-    (case the (kind g cond) of 
+    (case (kind g cond) of 
       ConstantNode condv \<Rightarrow> 
         RefNode (if (val_to_bool condv) then tb else fb) |
       _ \<Rightarrow> (if tb = fb then
@@ -137,14 +137,15 @@ text_raw \<open>\EndSnip\<close>
 
 lemma add_node_lookup:
   assumes "g' = add_node nid k g"
-  shows "kind g' nid = Some k"
-  using assms unfolding add_node.simps
-  using Rep_IRGraph_inverse kind.transfer by auto
+  shows "kind g' nid = k"
+  using assms unfolding add_node_def
+  using Rep_IRGraph_inverse kind.transfer
+  using add_node.rep_eq add_node_def kind.rep_eq map_upd_def node_kind_def by auto
 
 
 text_raw \<open>\Snip{IfNodeCreate}%\<close>
 lemma if_node_create:
-  assumes cv: "g m \<turnstile> cond (the (kind g cond)) \<mapsto> IntVal cv"
+  assumes cv: "g m \<turnstile> cond (kind g cond) \<mapsto> IntVal cv"
   assumes fresh: "nid \<notin> ids g" 
   assumes gif: "gif = add_node nid (IfNode cond tb fb) g"
   assumes gif_lookup: "gif = gif_prog sig"
@@ -155,17 +156,17 @@ lemma if_node_create:
   shows "\<exists>nid'. (gif_prog sig m \<turnstile> nid \<leadsto> nid') \<and> 
                 (gcreate_prog sig m \<turnstile> nid \<leadsto> nid')"
 text_raw \<open>\EndSnip\<close>
-proof (cases "\<exists> val . the (kind g cond) = ConstantNode val")
+proof (cases "\<exists> val . (kind g cond) = ConstantNode val")
   case True
   show ?thesis
   proof -
-    obtain val where val: "the (kind g cond) = ConstantNode val"
+    obtain val where val: "(kind g cond) = ConstantNode val"
       using True by blast
     have cond_exists: "cond \<in> ids g"
       using cv sorry
-    have if_kind: "kind gif nid = Some (IfNode cond tb fb)"
+    have if_kind: "kind gif nid = (IfNode cond tb fb)"
       using gif add_node_lookup by simp
-    have if_cv: "gif m \<turnstile> cond (the (kind gif cond)) \<mapsto> IntVal val"
+    have if_cv: "gif m \<turnstile> cond (kind gif cond) \<mapsto> IntVal val"
       using step.IfNode if_kind
       using True eval.ConstantNode gif fresh
       using stay_same cond_exists
@@ -177,7 +178,7 @@ proof (cases "\<exists> val . the (kind g cond) = ConstantNode val")
     qed
     have create_step: "(gcreate_prog, sig) \<turnstile> (nid,m,heap) \<rightarrow> (if val_to_bool val then tb else fb,m,heap)"
     proof -
-      have create_kind: "kind gcreate nid = Some (create_if g cond tb fb)"
+      have create_kind: "kind gcreate nid = (create_if g cond tb fb)"
         using gcreate add_node_lookup
         by blast
       have create_fun: "create_if g cond tb fb = RefNode (if val_to_bool val then tb else fb)"
@@ -195,12 +196,12 @@ next
   proof -
     have nid': "nid' = (if val_to_bool cv then tb else fb)"
       by (simp add: \<open>nid' = (if val_to_bool cv then tb else fb)\<close>)
-    have gif_kind: "kind gif nid = Some (IfNode cond tb fb)"
+    have gif_kind: "kind gif nid = (IfNode cond tb fb)"
       using add_node_lookup gif
       by blast
     have "nid \<noteq> cond"
       using cv fresh indep sorry
-    obtain cv2 where cv2: "gif m \<turnstile> cond (the (kind gif cond)) \<mapsto> cv2" 
+    obtain cv2 where cv2: "gif m \<turnstile> cond (kind gif cond) \<mapsto> cv2" 
       using \<open>nid \<noteq> cond\<close> cv gif indep
       using fresh sorry
     then have "IntVal cv = cv2"
@@ -210,21 +211,21 @@ next
     then have eval_gif: "((gif_prog, sig) \<turnstile> (nid,m,heap) \<rightarrow> (nid',m,heap))"
       using step.IfNode gif_kind nid' cv2 
       using gif_lookup by auto
-    have gcreate_kind: "kind gcreate nid = Some (create_if g cond tb fb)"
+    have gcreate_kind: "kind gcreate nid = (create_if g cond tb fb)"
       using gcreate add_node_lookup
       by blast
     have eval_gcreate: "(gcreate_prog, sig) \<turnstile> (nid,m,heap) \<rightarrow> (nid',m,heap)"
     proof (cases "tb = fb")
       case True
       have "create_if g cond tb fb = RefNode tb"
-        using not_const True by (cases "the (kind g cond)"; auto)
+        using not_const True by (cases "(kind g cond)"; auto)
       then show ?thesis
         using True gcreate_kind nid' step.RefNode
         by (simp add: gcreate_lookup)
     next
       case False
       have "create_if g cond tb fb = IfNode cond tb fb"
-        using not_const False by (cases "the (kind g cond)"; auto)
+        using not_const False by (cases "(kind g cond)"; auto)
       then show ?thesis
         using eval_gif gcreate gif
         using IfNode \<open>IntVal cv = cv2\<close> cv2 gcreate_lookup gif_kind nid' by auto
