ConditionalElimination.thy
@@ -1,0 +1,32 @@
+theory ConditionalElimination
+  imports
+    IREval
+    Stamp
+begin
+
+fun stamp :: "IRGraph \<Rightarrow> ID \<Rightarrow> Stamp" where
+  "stamp g nid = unrestricted (IntegerStamp 8 0 0)"
+
+fun wff_stamps :: "IRGraph \<Rightarrow> bool" where
+  "wff_stamps g = (\<forall> n \<in> ids g . 
+    (\<forall> v m . (g m \<turnstile> n (the (kind g n)) \<mapsto> v) \<and> valid_value (stamp g n) v))"
+
+lemma
+  assumes "joined = (join (stamp g x) (stamp g y))"
+  assumes "stamp_empty joined"
+  shows "\<nexists> v . valid_value joined v" 
+  using assms unfolding stamp_empty.simps
+  sorry
+
+lemma foldBinaryOpLogicJoin:
+  assumes "wff_stamps g"
+  assumes "is_IntegerStamp (stamp g x)"
+  assumes "is_IntegerStamp (stamp g y)"
+  assumes "kind g nid = (Some (IntegerEqualsNode x y))"
+  assumes "g m \<turnstile> nid (the (kind g nid)) \<mapsto> v"
+  assumes "stamp_empty (join (stamp g x) (stamp g y))"
+  shows "v = IntVal 0"
+  using eval.IntegerEqualsNode
+
+
+end
