IRGraphFrames.thy
@@ -55,7 +55,7 @@ inductive eval_uses:: "IRGraph \<Rightarrow> ID \<Rightarrow> ID \<Rightarrow> b
 
 
 fun eval_usages :: "IRGraph \<Rightarrow> ID \<Rightarrow> ID set" where
-  "eval_usages g nid = {n \<in> dom (Rep_IRGraph g) . eval_uses g nid n}"
+  "eval_usages g nid = {n \<in> ids g . eval_uses g nid n}"
 
 lemma eval_usages_self:
   assumes "nid \<in> ids g"
@@ -65,30 +65,31 @@ lemma eval_usages_self:
 
 lemma not_in_g: 
   assumes "nid \<notin> ids g"
-  shows "kind g nid = None"
+  shows "kind g nid = NoNode"
   using assms ids_some by blast
 
 lemma not_in_g_inp: 
   assumes "nid \<notin> ids g"
   shows "inp g nid = []"
 proof -
-  have k: "kind g nid = None" using assms not_in_g by blast
+  have k: "kind g nid = NoNode" using assms not_in_g by blast
   then show ?thesis by (simp add: k)
 qed
 
 lemma child_member:
-  assumes "Some n = kind g nid"
+  assumes "n = kind g nid"
+  assumes "n \<noteq> NoNode"
   assumes "List.member (inputs_of n) child"
   shows "child \<in> set (inp g nid)"
   unfolding inp.simps using assms
-  by (metis in_set_member option.simps(5)) 
+  by (metis in_set_member) 
 
 lemma child_member_in:
   assumes "nid \<in> ids g"
-  assumes "List.member (inputs_of (the (kind g nid))) child"
+  assumes "List.member (inputs_of (kind g nid)) child"
   shows "child \<in> set (inp g nid)"
   unfolding inp.simps using assms
-  by (metis child_member ids_some inp.elims option.exhaust_sel)
+  by (metis child_member ids_some inp.elims)
 
 
 (* Node inputs are not necessarily in ids g (unless wff_graph g).
@@ -100,7 +101,7 @@ proof -
   have "inp g nid \<noteq> []"
     using assms
     by (metis empty_iff empty_set)
-  then have "kind g nid \<noteq> None"
+  then have "kind g nid \<noteq> NoNode"
     using not_in_g_inp
     using ids_some by blast
   then show ?thesis
@@ -160,33 +161,35 @@ lemma usage_includes_inputs:
   using assms(1) assms(2) assms(3) by blast
 
 lemma elim_inp_set:
-  assumes "Some k = kind g nid"
+  assumes "k = kind g nid"
+  assumes "k \<noteq> NoNode"
   assumes "child \<in> set (inputs_of k)"
   shows "child \<in> set (inp g nid)"
-  using assms(1) assms(2)
-  by (metis inp.simps option.simps(5))
+  using assms by auto
 
+lemma eval_in_ids:
+  assumes "g m \<turnstile> nid (kind g nid) \<mapsto> v"
+  shows "nid \<in> ids g"
+  using assms by (cases "kind g nid = NoNode"; auto)
 
 (* Main theorem that we want. *)
 theorem stay_same:
-  assumes "kind g1 nid \<noteq> None"
   assumes nc: "unchanged (eval_usages g1 nid) g1 g2"
-  assumes g1: "g1 m \<turnstile> nid (the (kind g1 nid)) \<mapsto> v1"
+  assumes g1: "g1 m \<turnstile> nid (kind g1 nid) \<mapsto> v1"
   assumes wff: "wff_graph g1"
-  shows "g2 m \<turnstile> nid (the (kind g2 nid)) \<mapsto> v1"
+  shows "g2 m \<turnstile> nid (kind g2 nid) \<mapsto> v1"
 proof -
   have nid: "nid \<in> ids g1"
-    using not_in_g g1
-    by (meson assms(1))
+    using g1 eval_in_ids by simp
   then have "nid \<in> eval_usages g1 nid" 
     using eval_usages_self by blast
   then have kind_same: "kind g1 nid = kind g2 nid"
     using nc node_unchanged by blast 
   show ?thesis using g1 nid nc (* kind_same *)
-  proof (induct m nid "the (kind g1 nid)" v1 arbitrary: nid rule: "eval.induct")
+  proof (induct m nid "(kind g1 nid)" v1 arbitrary: nid rule: "eval.induct")
     print_cases
     case const: (ConstantNode val c m nid)
-    then have "the (kind g2 nid) = ConstantNode c"
+    then have "(kind g2 nid) = ConstantNode c"
       using kind_unchanged by metis
     then show ?case using eval.ConstantNode const.hyps(1) by metis
   next
@@ -195,7 +198,7 @@ proof -
       by (metis eval.ParameterNode kind_unchanged param.hyps(1) param.hyps(2) param.prems(1) param.prems(2))
   next
     case (PhiNode val m nida uv uu nid)
-    then have kind: "the (kind g2 nid) = (PhiNode nida uu)"
+    then have kind: "(kind g2 nid) = (PhiNode nida uu)"
       using kind_unchanged
       by metis
     then show ?case
@@ -203,7 +206,7 @@ proof -
       by metis
   next
     case (ValuePhiNode val m nida uw ux uy nid)
-    then have kind: "the (kind g2 nid) = ValuePhiNode nida ux uy"
+    then have kind: "(kind g2 nid) = ValuePhiNode nida ux uy"
       using kind_unchanged by metis
     then show ?case
       using eval.ValuePhiNode kind ValuePhiNode.hyps(1) by metis 
@@ -217,7 +220,7 @@ proof -
       using wff inp_in_g_wff by blast
     from inp_in have unc: "unchanged (eval_usages g1 child) g1 g2"
       using child_unchanged ValueProxyNode.prems(2) by metis
-    then have "g2 m \<turnstile> child (the (kind g2 child)) \<mapsto> val"
+    then have "g2 m \<turnstile> child (kind g2 child) \<mapsto> val"
       using ValueProxyNode.hyps(2) cin
       by blast
     then show ?case
@@ -225,10 +228,10 @@ proof -
   next
     case (AbsNode m x v _ nid)
     then have "unchanged (eval_usages g1 x) g1 g2"
-      by (metis child_unchanged elim_inp_set ids_some inputs_of.simps(1) list.set_intros(1) option.exhaust_sel)
-    then have "g2 m \<turnstile> x (the (kind g2 x)) \<mapsto> IntVal v"
+      by (metis child_unchanged elim_inp_set ids_some inputs_of.simps(1) list.set_intros(1))
+    then have "g2 m \<turnstile> x (kind g2 x) \<mapsto> IntVal v"
       using AbsNode.hyps(1) AbsNode.hyps(2) not_in_g
-      by (metis AbsNode.hyps(3) AbsNode.prems(1) elim_inp_set ids_some inp_in_g_wff inputs_of.simps(1) list.set_intros(1) option.exhaust_sel wff)
+      by (metis AbsNode.hyps(3) AbsNode.prems(1) elim_inp_set ids_some inp_in_g_wff inputs_of.simps(1) list.set_intros(1) wff)
     then show ?case
       by (metis AbsNode.hyps(3) AbsNode.prems(1) AbsNode.prems(2) eval.AbsNode kind_unchanged)
   next
@@ -240,10 +243,10 @@ proof -
       using wff inp_in_g_wff by blast
     from xinp child_unchanged Node.prems(2)
       have ux: "unchanged (eval_usages g1 x) g1 g2" by blast
-    have x1:"g1 m \<turnstile> x (the (kind g1 x)) \<mapsto> IntVal v"
+    have x1:"g1 m \<turnstile> x (kind g1 x) \<mapsto> IntVal v"
       using Node.hyps(1) Node.hyps(2)
       by blast
-    have x2: "g2 m \<turnstile> x (the (kind g2 x)) \<mapsto> IntVal v"
+    have x2: "g2 m \<turnstile> x (kind g2 x) \<mapsto> IntVal v"
       using kind_unchanged ux xin Node.hyps
       by blast
     then show ?case
@@ -252,90 +255,90 @@ proof -
   next
     case node:(AddNode m x v1 y v2 nid)
     then have ux: "unchanged (eval_usages g1 x) g1 g2"
-      by (metis child_unchanged ids_some inp.simps inputs_of.simps(9) list.set_intros(1) option.exhaust_sel option.simps(5))
-    then have x: "g1 m \<turnstile> x (the (kind g1 x)) \<mapsto> IntVal v1"
+      by (metis child_unchanged inp.simps inputs_of.simps(9) list.set_intros(1))
+    then have x: "g1 m \<turnstile> x (kind g1 x) \<mapsto> IntVal v1"
       using node.hyps(1) by blast
     have uy: "unchanged (eval_usages g1 y) g1 g2"
       by (metis IRNodes.inputs_of_AddNode child_member_in child_unchanged member_rec(1) node.hyps(5) node.prems(1) node.prems(2))
-    have y: "g1 m \<turnstile> y (the (kind g1 y)) \<mapsto> IntVal v2"
+    have y: "g1 m \<turnstile> y (kind g1 y) \<mapsto> IntVal v2"
       using node.hyps(3) by blast
     show ?case
       using node.hyps node.prems ux x uy y
-      by (metis AddNode ids_some inp.simps inp_in_g_wff inputs_of_AddNode kind_unchanged list.set_intros(1) option.case(2) option.exhaust_sel set_subset_Cons subset_iff wff)
+      by (metis AddNode inp.simps inp_in_g_wff inputs_of_AddNode kind_unchanged list.set_intros(1) set_subset_Cons subset_iff wff)
   next
     case node:(SubNode m x v1 y v2 nid)
     then have ux: "unchanged (eval_usages g1 x) g1 g2"
       by (metis child_member_in child_unchanged inputs_of_SubNode member_rec(1))
-    then have x: "g1 m \<turnstile> x (the (kind g1 x)) \<mapsto> IntVal v1"
+    then have x: "g1 m \<turnstile> x (kind g1 x) \<mapsto> IntVal v1"
       using node.hyps(1) by blast
     from node have uy: "unchanged (eval_usages g1 y) g1 g2"
       by (metis child_member_in child_unchanged inputs_of_SubNode member_rec(1))
-    have y: "g1 m \<turnstile> y (the (kind g1 y)) \<mapsto> IntVal v2"
+    have y: "g1 m \<turnstile> y (kind g1 y) \<mapsto> IntVal v2"
       using node.hyps(3) by blast
     show ?case
       using node.hyps node.prems ux x uy y
-      by (metis SubNode inp.simps inputs_of_SubNode kind_unchanged list.set_intros(1) option.exhaust_sel option.simps(5) set_subset_Cons subsetD wff wff_graph.elims(2))
+      by (metis SubNode inp.simps inputs_of_SubNode kind_unchanged list.set_intros(1) set_subset_Cons subsetD wff wff_graph.elims(2))
   next
     case node:(MulNode m x v1 y v2 nid)
     then have ux: "unchanged (eval_usages g1 x) g1 g2"
       by (metis child_member_in child_unchanged inputs_of_MulNode member_rec(1))
-    then have x: "g1 m \<turnstile> x (the (kind g1 x)) \<mapsto> IntVal v1"
+    then have x: "g1 m \<turnstile> x (kind g1 x) \<mapsto> IntVal v1"
       using node.hyps(1) by blast
     from node have uy: "unchanged (eval_usages g1 y) g1 g2"
       by (metis child_member_in child_unchanged inputs_of_MulNode member_rec(1))
-    have y: "g1 m \<turnstile> y (the (kind g1 y)) \<mapsto> IntVal v2"
+    have y: "g1 m \<turnstile> y (kind g1 y) \<mapsto> IntVal v2"
       using node.hyps(3) by blast
     show ?case
       using node.hyps node.prems ux x uy y
-      by (metis MulNode inp.simps inputs_of_MulNode kind_unchanged list.set_intros(1) option.exhaust_sel option.simps(5) set_subset_Cons subsetD wff wff_graph.elims(2))
+      by (metis MulNode inp.simps inputs_of_MulNode kind_unchanged list.set_intros(1) set_subset_Cons subsetD wff wff_graph.elims(2))
   next
     case node:(AndNode m x v1 y v2 nid)
     then have ux: "unchanged (eval_usages g1 x) g1 g2"
       by (metis child_member_in child_unchanged inputs_of_AndNode member_rec(1))
-    then have x: "g1 m \<turnstile> x (the (kind g1 x)) \<mapsto> IntVal v1"
+    then have x: "g1 m \<turnstile> x (kind g1 x) \<mapsto> IntVal v1"
       using node.hyps(1) by blast
     from node have uy: "unchanged (eval_usages g1 y) g1 g2"
       by (metis child_member_in child_unchanged inputs_of_AndNode member_rec(1))
-    have y: "g1 m \<turnstile> y (the (kind g1 y)) \<mapsto> IntVal v2"
+    have y: "g1 m \<turnstile> y (kind g1 y) \<mapsto> IntVal v2"
       using node.hyps(3) by blast
     show ?case
       using node.hyps node.prems ux x uy y
-      by (metis AndNode inp.simps inputs_of_AndNode kind_unchanged list.set_intros(1) option.exhaust_sel option.simps(5) set_subset_Cons subsetD wff wff_graph.elims(2))
+      by (metis AndNode inp.simps inputs_of_AndNode kind_unchanged list.set_intros(1) set_subset_Cons subsetD wff wff_graph.elims(2))
   next
     case node: (OrNode m x v1 y v2 nid)
     then have ux: "unchanged (eval_usages g1 x) g1 g2"
       by (metis child_member_in child_unchanged inputs_of_OrNode member_rec(1))
-    then have x: "g1 m \<turnstile> x (the (kind g1 x)) \<mapsto> IntVal v1"
+    then have x: "g1 m \<turnstile> x (kind g1 x) \<mapsto> IntVal v1"
       using node.hyps(1) by blast
     from node have uy: "unchanged (eval_usages g1 y) g1 g2"
       by (metis child_member_in child_unchanged inputs_of_OrNode member_rec(1))
-    have y: "g1 m \<turnstile> y (the (kind g1 y)) \<mapsto> IntVal v2"
+    have y: "g1 m \<turnstile> y (kind g1 y) \<mapsto> IntVal v2"
       using node.hyps(3) by blast
     show ?case
       using node.hyps node.prems ux x uy y
-      by (metis OrNode inp.simps inputs_of_OrNode kind_unchanged list.set_intros(1) option.exhaust_sel option.simps(5) set_subset_Cons subsetD wff wff_graph.elims(2))
+      by (metis OrNode inp.simps inputs_of_OrNode kind_unchanged list.set_intros(1) set_subset_Cons subsetD wff wff_graph.elims(2))
   next
     case node: (XorNode m x v1 y v2 nid)
     then have ux: "unchanged (eval_usages g1 x) g1 g2"
       by (metis child_member_in child_unchanged inputs_of_XorNode member_rec(1))
-    then have x: "g1 m \<turnstile> x (the (kind g1 x)) \<mapsto> IntVal v1"
+    then have x: "g1 m \<turnstile> x (kind g1 x) \<mapsto> IntVal v1"
       using node.hyps(1) by blast
     from node have uy: "unchanged (eval_usages g1 y) g1 g2"
       by (metis child_member_in child_unchanged inputs_of_XorNode member_rec(1))
-    have y: "g1 m \<turnstile> y (the (kind g1 y)) \<mapsto> IntVal v2"
+    have y: "g1 m \<turnstile> y (kind g1 y) \<mapsto> IntVal v2"
       using node.hyps(3) by blast
     show ?case
       using node.hyps node.prems ux x uy y
-      by (metis XorNode inp.simps inputs_of_XorNode kind_unchanged list.set_intros(1) option.exhaust_sel option.simps(5) set_subset_Cons subsetD wff wff_graph.elims(2))
+      by (metis XorNode inp.simps inputs_of_XorNode kind_unchanged list.set_intros(1) set_subset_Cons subsetD wff wff_graph.elims(2))
   next
     case node: (IntegerEqualsNode m x v1 y v2 val nid)
     then have ux: "unchanged (eval_usages g1 x) g1 g2"
       by (metis child_member_in child_unchanged inputs_of_IntegerEqualsNode member_rec(1))
-    then have x: "g1 m \<turnstile> x (the (kind g1 x)) \<mapsto> IntVal v1"
+    then have x: "g1 m \<turnstile> x (kind g1 x) \<mapsto> IntVal v1"
       using node.hyps(1) by blast
     from node have uy: "unchanged (eval_usages g1 y) g1 g2"
       by (metis child_member_in child_unchanged inputs_of_IntegerEqualsNode member_rec(1))
-    have y: "g1 m \<turnstile> y (the (kind g1 y)) \<mapsto> IntVal v2"
+    have y: "g1 m \<turnstile> y (kind g1 y) \<mapsto> IntVal v2"
       using node.hyps(3) by blast
     show ?case
       using node.hyps node.prems ux x uy y
@@ -344,11 +347,11 @@ proof -
     case node: (IntegerLessThanNode m x v1 y v2 val nid)
     then have ux: "unchanged (eval_usages g1 x) g1 g2"
       by (metis child_member_in child_unchanged inputs_of_IntegerLessThanNode member_rec(1))
-    then have x: "g1 m \<turnstile> x (the (kind g1 x)) \<mapsto> IntVal v1"
+    then have x: "g1 m \<turnstile> x (kind g1 x) \<mapsto> IntVal v1"
       using node.hyps(1) by blast
     from node have uy: "unchanged (eval_usages g1 y) g1 g2"
       by (metis child_member_in child_unchanged inputs_of_IntegerLessThanNode member_rec(1))
-    have y: "g1 m \<turnstile> y (the (kind g1 y)) \<mapsto> IntVal v2"
+    have y: "g1 m \<turnstile> y (kind g1 y) \<mapsto> IntVal v2"
       using node.hyps(3) by blast
     show ?case
       using node.hyps node.prems ux x uy y
@@ -357,16 +360,16 @@ proof -
     case node: (ShortCircuitOrNode m x v1 y v2 val nid)
     then have ux: "unchanged (eval_usages g1 x) g1 g2"
       by (metis child_member_in child_unchanged inputs_of_ShortCircuitOrNode member_rec(1))
-    then have x: "g1 m \<turnstile> x (the (kind g1 x)) \<mapsto> IntVal v1"
+    then have x: "g1 m \<turnstile> x (kind g1 x) \<mapsto> IntVal v1"
       using node.hyps(1) by blast
     from node have uy: "unchanged (eval_usages g1 y) g1 g2"
       by (metis child_member_in child_unchanged inputs_of_ShortCircuitOrNode member_rec(1))
-    have y: "g1 m \<turnstile> y (the (kind g1 y)) \<mapsto> IntVal v2"
+    have y: "g1 m \<turnstile> y (kind g1 y) \<mapsto> IntVal v2"
       using node.hyps(3) by blast
-    have x2: "g2 m \<turnstile> x (the (kind g2 x)) \<mapsto> IntVal v1"
-      by (metis inp.simps inputs_of_ShortCircuitOrNode list.set_intros(1) node.hyps(2) node.hyps(6) node.prems(1) option.exhaust_sel option.simps(5) subsetD ux wff wff_graph.elims(2))
-    have y2: "g2 m \<turnstile> y (the (kind g2 y)) \<mapsto> IntVal v2"
-      by (metis basic_trans_rules(31) inp.simps inputs_of.simps(50) list.set_intros(1) node.hyps(4) node.hyps(6) node.prems(1) option.exhaust_sel option.simps(5) set_subset_Cons uy wff wff_graph.elims(2))
+    have x2: "g2 m \<turnstile> x (kind g2 x) \<mapsto> IntVal v1"
+      by (metis inp.simps inputs_of_ShortCircuitOrNode list.set_intros(1) node.hyps(2) node.hyps(6) node.prems(1) subsetD ux wff wff_graph.elims(2))
+    have y2: "g2 m \<turnstile> y (kind g2 y) \<mapsto> IntVal v2"
+      by (metis basic_trans_rules(31) inp.simps inputs_of.simps(50) list.set_intros(1) node.hyps(4) node.hyps(6) node.prems(1) set_subset_Cons uy wff wff_graph.elims(2))
     show ?case
       using node.hyps node.prems ux x uy y x2 y2
       by (metis ShortCircuitOrNode kind_unchanged)
@@ -374,8 +377,8 @@ proof -
     case node: (LogicNegationNode m x v1 val nida nid)
     then have ux: "unchanged (eval_usages g1 x) g1 g2"
       by (metis child_member_in child_unchanged inputs_of_LogicNegationNode member_rec(1))
-    then have x:"g2 m \<turnstile> x (the (kind g2 x)) \<mapsto> IntVal v1"
-      by (metis ids_some inp.simps inp_in_g_wff inputs_of.simps(34) list.set_intros(1) node.hyps(2) node.hyps(4) node.prems(1) option.exhaust_sel option.simps(5) wff)
+    then have x:"g2 m \<turnstile> x (kind g2 x) \<mapsto> IntVal v1"
+      by (metis inp.simps inp_in_g_wff inputs_of.simps(34) list.set_intros(1) node.hyps(2) node.hyps(4) wff)
     then show ?case
       by (metis LogicNegationNode kind_unchanged node.hyps(3) node.hyps(4) node.prems(1) node.prems(2))
   next
@@ -384,24 +387,24 @@ proof -
       by (metis IRNodes.inputs_of_ConditionalNode child_member_in member_rec(1) node.hyps(8) node.prems(1))
     then have "unchanged (eval_usages g1 condition) g1 g2"
       using child_unchanged node.prems(2) by blast
-    then have cond: "g2 m \<turnstile> condition (the (kind g2 condition)) \<mapsto> IntVal cond"
+    then have cond: "g2 m \<turnstile> condition (kind g2 condition) \<mapsto> IntVal cond"
       using node c inp_in_g_wff wff by blast
 
     have t: "trueExp \<in> set(inp g1 nid)"
       by (metis IRNodes.inputs_of_ConditionalNode child_member_in member_rec(1) node.hyps(8) node.prems(1))
     then have utrue: "unchanged (eval_usages g1 trueExp) g1 g2"
       using node.prems(2) child_unchanged by blast
-    then have trueVal: "g2 m \<turnstile> trueExp (the (kind g2 trueExp)) \<mapsto> IntVal(trueVal)"
+    then have trueVal: "g2 m \<turnstile> trueExp (kind g2 trueExp) \<mapsto> IntVal(trueVal)"
       using node.hyps node t inp_in_g_wff wff by blast
 
     have f: "falseExp \<in> set(inp g1 nid)"
       by (metis IRNodes.inputs_of_ConditionalNode child_member_in member_rec(1) node.hyps(8) node.prems(1))
     then have ufalse: "unchanged (eval_usages g1 falseExp) g1 g2"
       using node.prems(2) child_unchanged by blast
-    then have falseVal: "g2 m \<turnstile> falseExp (the (kind g2 falseExp)) \<mapsto> IntVal(falseVal)"
+    then have falseVal: "g2 m \<turnstile> falseExp (kind g2 falseExp) \<mapsto> IntVal(falseVal)"
       using node.hyps node f inp_in_g_wff wff by blast
 
-    have "g2 m \<turnstile> nid (the (kind g2 nid)) \<mapsto> val"
+    have "g2 m \<turnstile> nid (kind g2 nid) \<mapsto> val"
       using kind_same trueVal falseVal cond
       by (metis ConditionalNode kind_unchanged node.hyps(7) node.hyps(8) node.prems(1) node.prems(2))
     then show ?case
@@ -411,7 +414,7 @@ proof -
     case (RefNode m x val nid)
     have x: "x \<in> set(inp g1 nid)"
       by (metis IRNodes.inputs_of_RefNode RefNode.hyps(3) RefNode.prems(1) child_member_in member_rec(1))
-    then have ref: "g2 m \<turnstile> x (the (kind g2 x)) \<mapsto> val"
+    then have ref: "g2 m \<turnstile> x (kind g2 x) \<mapsto> val"
       using RefNode.hyps(2) RefNode.prems(2) child_unchanged inp_in_g_wff wff by blast
     then show ?case
       by (metis RefNode.hyps(3) RefNode.prems(1) RefNode.prems(2) eval.RefNode kind_unchanged)
@@ -423,11 +426,11 @@ proof -
     case (SignedDivNode m x v1 y v2 nid zeroCheck frameState nex)
     have xinp: "x \<in> set(inp g1 nid)"
       by (metis IRNodes.inputs_of_SignedDivNode SignedDivNode.hyps(5) SignedDivNode.prems(1) append_Cons child_member_in member_rec(1))
-    from xinp have x: "g2 m \<turnstile> x (the (kind g2 x)) \<mapsto> IntVal v1"
+    from xinp have x: "g2 m \<turnstile> x (kind g2 x) \<mapsto> IntVal v1"
       using SignedDivNode child_unchanged inp_in_g_wff wff by blast
     have yinp: "y \<in> set(inp g1 nid)"
       by (metis IRNodes.inputs_of_SignedDivNode SignedDivNode.hyps(5) SignedDivNode.prems(1) append_Cons child_member_in member_rec(1))
-    from yinp have y: "g2 m \<turnstile> y (the (kind g2 y)) \<mapsto> IntVal v2"
+    from yinp have y: "g2 m \<turnstile> y (kind g2 y) \<mapsto> IntVal v2"
       using SignedDivNode child_unchanged inp_in_g_wff wff by blast
     from x y show ?case
       by (metis SignedDivNode.hyps(5) SignedDivNode.prems(1) SignedDivNode.prems(2) eval.SignedDivNode kind_unchanged)
