IRNodes.thy
@@ -110,13 +110,9 @@ datatype (discs_sels) IRNode =
   (* Manually added *)
   | SubstrateMethodCallTargetNode (ir_targetMethod: string) (ir_arguments: "INPUT list") 
   | RefNode (ir_ref:ID)
+  | NoNode
 
 (* The '(discs_sels)' above automatically generates (is_StartNode _) etc.*)
-
-
-text \<open>isType is used to compose a type selector function for a possibly empty IRNode\<close>
-fun isType :: "(IRNode \<Rightarrow> bool) \<Rightarrow> IRNode option \<Rightarrow> bool" where
-  "isType nodeType node = (case node of None \<Rightarrow> False | Some n \<Rightarrow> nodeType n)"
 
 
 text \<open>Class inheritance functions to determine if a node is extended from another\<close>
@@ -305,7 +301,8 @@ fun inputs_of :: "IRNode \<Rightarrow> ID list" where
 (* nodeout *)
 
   inputs_of_SubstrateMethodCallTargetNode: "inputs_of (SubstrateMethodCallTargetNode targetMethod args) = args" |
-  inputs_of_RefNode: "inputs_of (RefNode ref) = [ref]"
+  inputs_of_RefNode: "inputs_of (RefNode ref) = [ref]" |
+  inputs_of_NoNode: "inputs_of (NoNode) = []"
 
 (* nodeout: isabelle-succs *)
 fun successors_of :: "IRNode \<Rightarrow> ID list" where
@@ -436,7 +433,8 @@ fun successors_of :: "IRNode \<Rightarrow> ID list" where
 (* nodeout *)
 
   successors_of_SubstrateMethodCallTargetNode: "successors_of (SubstrateMethodCallTargetNode targetMethod args) = []" |
-  successors_of_RefNode: "successors_of (RefNode ref) = []"
+  successors_of_RefNode: "successors_of (RefNode ref) = []" |
+  successors_of_NoNode: "successors_of (NoNode) = []"
 
 
 
